TCR/Data/Vector.lean
@@ -5,41 +5,52 @@ Authors: Markus Himmel
 -/
 module
 
+namespace Vector
+
 @[simp]
-public theorem Vector.getD_mk {a : Array α} {n : Nat} (h : a.size = n) {m : Nat} {b : α} :
+public theorem getD_mk {a : Array α} {n : Nat} (h : a.size = n) {m : Nat} {b : α} :
     (Vector.mk a h).getD m b = a.getD m b := rfl
 
 @[simp]
-public theorem Vector.getD_eq_getD_getElem? {v : Vector α n} {m : Nat} {a : α} :
+public theorem getD_eq_getD_getElem? {v : Vector α n} {m : Nat} {a : α} :
     v.getD m a = v[m]?.getD a := by
   cases v; simp
 
-public theorem Vector.getD_set_ne {v : Vector α n} {m k : Nat} {hm} {a b : α} (hmk : m ≠ k) :
+public theorem getD_set_ne {v : Vector α n} {m k : Nat} {hm} {a b : α} (hmk : m ≠ k) :
     (v.set m a hm).getD k b = v.getD k b := by
   simp [Vector.getElem?_set_ne _ hmk]
 
 /-- Applies the function `f` to the `i`-th element of `v`, provided `i < n`. Otherwise, returns
 `v` unmodified. -/
-public def Vector.modify (v : Vector α n) (i : Nat) (f : α → α) : Vector α n where
+public def modify (v : Vector α n) (i : Nat) (f : α → α) : Vector α n where
   toArray := v.toArray.modify i f
   size_toArray := by simp
 
 @[simp]
-public theorem Vector.toArray_modify {v : Vector α n} {i : Nat} {f : α → α} :
+public theorem toArray_modify {v : Vector α n} {i : Nat} {f : α → α} :
     (v.modify i f).toArray = v.toArray.modify i f := (rfl)
 
 @[simp]
-public theorem Vector.modify_mk {a : Array α} (hn : a.size = n) {i : Nat} {f : α → α} :
+public theorem modify_mk {a : Array α} (hn : a.size = n) {i : Nat} {f : α → α} :
     (Vector.mk a hn).modify i f = Vector.mk (a.modify i f) (by simp [hn]) := (rfl)
 
 @[simp]
-public theorem Vector.modify_cast {h : n = m} {v : Vector α n} {i : Nat} {f : α → α} :
+public theorem modify_cast {h : n = m} {v : Vector α n} {i : Nat} {f : α → α} :
     (v.cast h).modify i f = (v.modify i f).cast h := (rfl)
 
-public theorem Vector.getElem_modify {f : α → α} {v : Vector α n} {j i : Nat} {h} :
+public theorem getElem_modify {f : α → α} {v : Vector α n} {j i : Nat} {h} :
     (v.modify j f)[i]'h = if j = i then f v[i] else v[i] := by
   cases v
   simp [Array.getElem_modify]
 
-public theorem Vector.getElem_modify_of_ne {j : Nat} {v : Vector α n} {i : Nat} (hi : i ≠ j) (f : α → α) (hj) : (v.modify i f)[j] = v[j] := by
+public theorem getElem_modify_of_ne {j : Nat} {v : Vector α n} {i : Nat} (hi : i ≠ j) (f : α → α) (hj) : (v.modify i f)[j] = v[j] := by
   simp [getElem_modify, hi]
+
+public theorem extract_eq_cast_empty {i j : Nat} {v : Vector α n} (h : min j n ≤ i) : v.extract i j = #v[].cast (by grind) := by
+  simpa [← Vector.toArray_inj]
+
+@[simp]
+public theorem cast_replicate {n m : Nat} (h : n = m) (a : α) : (Vector.replicate n a).cast h = Vector.replicate m a := by
+  cases h; simp
+
+end Vector
