TCR/Data/SegmentTree/Lemmas.lean
@@ -1,0 +1,102 @@
+/-
+Copyright (c) 2025 Markus Himmel. All rights reserved.
+Released under Apache 2.0 license as described in the file LICENSE.
+Authors: Markus Himmel
+-/
+module
+
+public import TCR.Data.SegmentTree.Basic
+import all TCR.Data.SegmentTree.Basic
+import TCR.Data.SegmentTree.WF
+
+/-!
+# Segment tree lemmas
+
+This file characterizes segment tree modification operations in terms of `underlying`, and
+proves an extensionality theorem for segment trees.
+-/
+
+namespace TCR.SegmentTree
+
+namespace Impl
+
+theorem getElem_eq_getElem_underlying {v : Vector α (2 * n)} {i : Nat} {hi : i < 2 * n} (hi' : n ≤ i) :
+    v[i] = (underlying v)[i - n] := by
+  simp [underlying]
+  grind
+
+theorem getElem?_eq_getElem?_underlying {v : Vector α (2 * n)} {i : Nat} (hi' : n ≤ i) :
+    v[i]? = (underlying v)[i - n]? := by
+  simp [underlying]
+  grind [Vector.getElem?_extract]
+
+@[simp]
+theorem underlying_mkSegmentTree {op : α → α → α} {neutral : α} {v : Vector α n} :
+    underlying (mkSegmentTree op neutral v) = v := by
+  rw [mkSegmentTree]
+  split
+  · simp_all [underlying]
+  suffices ∀ (vec : Vector α (2 * n)) idx hidx,
+      (mkSegmentTree.loop op vec idx hidx).extract n (2 * n) = vec.extract n (2 * n) by
+    simp [underlying, this]
+    grind
+  intro vec idx hidx
+  fun_induction mkSegmentTree.loop <;> grind
+
+theorem IsSegmentTree.underlying_inj (v v' : Vector α (2 * n))
+    (hv : IsSegmentTree op neutral v) (hv' : IsSegmentTree op neutral v')
+    (h : underlying v = underlying v') : v = v' := by
+  suffices ∀ i, (h : i < n - 1) → v[n - i - 1] = v'[n - i - 1] by
+    ext i hi
+    have := this (n - i - 1)
+    have := hv.zero_eq
+    have := hv'.zero_eq
+    grind [getElem_eq_getElem_underlying]
+  intro i hi
+  induction i using Nat.strongRecOn with
+  | ind i ih =>
+    rw [hv.op_eq _ (by grind) (by grind), hv'.op_eq _ (by grind) (by grind)]
+    have := ih (2 * i + 1 - n)
+    have := ih (2 * i - n)
+    grind (splits := 12) [getElem_eq_getElem_underlying]
+
+@[simp]
+theorem underlying_modify {op : α → α → α} {v : Vector α (2 * n)} {i : Nat} {hi : i < n} {f : α → α} :
+    underlying (modify op v i hi f) = (underlying v).modify i f := by
+  suffices ∀ (vec : Vector α (2 * n)) idx hidx, underlying (modify.loop op i hi vec idx hidx) = underlying vec by
+    simp only [modify, this]
+    simp only [underlying, Vector.modify_cast, Vector.cast_eq_cast, Vector.cast_rfl]
+    ext j hj
+    simp [Vector.getElem_modify]
+  intro vec idx hidx
+  fun_induction modify.loop with grind [underlying]
+
+@[simp]
+theorem underlying_mkEmpty {neutral : α} {n : Nat} : underlying (mkEmpty neutral n) = Vector.replicate n neutral := by
+  simp [underlying, mkEmpty]
+
+end Impl
+
+@[simp]
+theorem underlying_ofVector {op : α → α → α} {neutral : α} {v : Vector α n} :
+    (SegmentTree.ofVector op neutral v).underlying = v :=
+  Impl.underlying_mkSegmentTree
+
+@[simp]
+theorem underlying_modify {op : α → α → α} {neutral : α} {t : SegmentTree op neutral n}
+    {i : Nat} {hi : i < n} {f : α → α} : (t.modify i hi f).underlying = t.underlying.modify i f :=
+  Impl.underlying_modify
+
+@[simp]
+theorem underlying_empty {op : α → α → α} {neutral : α} {n : Nat} :
+    (empty op neutral n).underlying = Vector.replicate n neutral :=
+  Impl.underlying_mkEmpty
+
+@[ext]
+theorem ext {op : α → α → α} {neutral : α} [Std.LawfulRightIdentity op neutral] {t t' : SegmentTree op neutral n} :
+    t.underlying = t'.underlying → t = t' := by
+  rcases t with ⟨t, ht⟩
+  rcases t' with ⟨t', ht'⟩
+  simpa using Impl.IsSegmentTree.underlying_inj _ _ ht.out ht'.out
+
+end TCR.SegmentTree
