TCR/Data/SegmentTree/Query.lean
@@ -1,0 +1,66 @@
+/-
+Copyright (c) 2025 Markus Himmel. All rights reserved.
+Released under Apache 2.0 license as described in the file LICENSE.
+Authors: Markus Himmel
+-/
+module
+
+import TCR.Data.Vector
+
+/-!
+# Verification of the segment tree `query` operation (WIP)
+
+This file will contain the internal part of the verification of the `query` operation on segment trees.
+The final user-facing lemma will appear in `TCR.Data.SegmentTree.Lemmas`.
+-/
+
+namespace TCR.SegmentTree
+
+namespace Impl
+
+/-- Returns the leftmost node reachable from node `i` in the implicit tree of size `n`. -/
+def leftmost (n i : Nat) : Nat :=
+  if i = 0 then
+    0
+  else if n ≤ i then
+    i
+  else
+    leftmost n (2 * i)
+
+@[simp]
+theorem leftmost_zero {n : Nat} : leftmost n 0 = 0 := by
+  simp [leftmost]
+
+theorem leftmost_eq_self {n i : Nat} (hi : 0 < i) (hni : n ≤ i) : leftmost n i = i := by
+  grind [leftmost]
+
+theorem leftmost_eq_leftmost_two_mul {n i : Nat} (hi : 0 < i) (hni : i < n) : leftmost n i = leftmost n (2 * i) := by
+  grind [leftmost]
+
+/-- `IsFold op neutral v l r a` is shorthand for the fact that `a` is obtained by folding `op` over `v[l...<r]`. -/
+def IsFold (op : α → α → α) (neutral : α) (v : Vector α k) (l r : Nat) (a : α) : Prop :=
+  a = (v.extract l r).foldl op neutral
+
+theorem isFold_iff {op : α → α → α} {neutral : α} {v : Vector α k} {l r : Nat} {a : α} :
+    IsFold op neutral v l r a ↔ a = (v.extract l r).foldl op neutral := Iff.rfl
+
+theorem IsFold.base {op : α → α → α} {neutral : α} {v : Vector α k} {l} : IsFold op neutral v l l neutral := by
+  simp [isFold_iff, Vector.extract_eq_cast_empty (Nat.min_le_left l k)]
+
+theorem Array.extract_eq_extract_append_extract (l r : Nat) {a : Array α} (m : Nat) (hl : l ≤ m) (hr : m ≤ r) :
+    a.extract l r = a.extract l m ++ a.extract m r := by
+  rw [Array.extract_append_extract, Nat.min_eq_left hl, Nat.max_eq_right hr]
+
+theorem IsFold.concat {op : α → α → α} {neutral : α} [Std.Associative op] [Std.LawfulRightIdentity op neutral]
+    {v : Vector α k} {l m r} {a b : α} (hlm : l ≤ m) (hmr : m ≤ r) :
+    IsFold op neutral v l m a → IsFold op neutral v m r b → IsFold op neutral v l r (op a b) := by
+  simp only [isFold_iff, isFold_iff]
+  rintro rfl rfl
+  rw [← Vector.foldl_assoc (op := op), Std.LawfulRightIdentity.right_id (op := op),
+    ← Vector.foldl_append, Vector.extract_append_extract]
+  rcases v with ⟨a, ha⟩
+  simp [Nat.min_eq_left hlm, Nat.max_eq_right hmr]
+
+end Impl
+
+end TCR.SegmentTree
