TCR/Data/SegmentTree/WF.lean
@@ -1,0 +1,75 @@
+/-
+Copyright (c) 2025 Markus Himmel. All rights reserved.
+Released under Apache 2.0 license as described in the file LICENSE.
+Authors: Markus Himmel
+-/
+module
+
+public import TCR.Data.SegmentTree.Basic
+import all TCR.Data.SegmentTree.Basic
+
+/-!
+# Well-formedness of segment trees
+
+In this file we prove the all segment tree operations preserve well-formedness.
+-/
+
+namespace TCR.SegmentTree
+
+namespace Impl
+
+theorem isSegmentTree_mkSegmentTree {op : α → α → α} {neutral : α} {v : Vector α n} :
+    IsSegmentTree op neutral (mkSegmentTree op neutral v) := by
+  rw [mkSegmentTree]
+  split
+  · refine ⟨by simp_all, by simp_all⟩
+  · refine loop _ _ ?_ (by grind)
+    simp_all [Array.getElem_append]
+where
+  loop {vec : Vector α (2 * n)} (idx : Nat) (hidx : idx < n)
+      (h₀ : vec[0] = neutral)
+      (h : ∀ idx', 0 < idx' → idx < idx' → (h : idx' < n) →
+        vec[idx'] = op vec[2 * idx'] vec[2 * idx' + 1]) :
+      IsSegmentTree op neutral (mkSegmentTree.loop op vec idx hidx) := by
+    fun_induction mkSegmentTree.loop with
+    | case1 => exact ⟨by simp_all, by simpa using h⟩
+    | case2 vec idx' hidx ih =>
+      refine ih ?_ (fun idx'' h₁ h₂ h₃ => ?_)
+      · rw [Vector.getElem_set_ne _ _ (by omega), h₀]
+      · rw [Vector.getElem_set]
+        split
+        · rename_i hx
+          subst hx
+          grind [Vector.getElem_set_ne]
+        · grind [Vector.getElem_set_ne]
+
+theorem IsSegmentTree.modify {op : α → α → α} {neutral : α} {v : Vector α (2 * n)} (hv : IsSegmentTree op neutral v)
+    {i : Nat} (hi : i < n) (f : α → α) : IsSegmentTree op neutral (modify op v i hi f) := by
+  rw [Impl.modify]
+  apply loop <;> grind [Vector.getElem_modify_of_ne, IsSegmentTree.zero_eq, IsSegmentTree.op_eq]
+where
+  loop {vec : Vector α (2 * n)} {idx hidx₀ hidx} (h₀ : vec[0] = neutral)
+      (h : ∀ (i : Nat) (_ : 0 < i) (hi : i < n) (_ : i ≠ idx), vec[i] = op vec[2 * i] vec[2 * i + 1]) :
+      IsSegmentTree op neutral (modify.loop op i hi vec idx hidx) := by
+    fun_induction modify.loop with grind [IsSegmentTree]
+
+theorem isSegmentTree_mkEmpty {op : α → α → α} {neutral : α} [Std.LawfulRightIdentity op neutral] {n : Nat} :
+    IsSegmentTree op neutral (mkEmpty neutral n) where
+  zero_eq h := by simp [mkEmpty]
+  op_eq i hi₀ hi := by simp [mkEmpty, Std.LawfulRightIdentity.right_id]
+
+/-- A well-formed segment tree has the segment tree property. -/
+public theorem WF.out {op : α → α → α} {neutral : α} [Std.LawfulRightIdentity op neutral] :
+    {v : Vector α (2 * n)} → Impl.WF op neutral v → IsSegmentTree op neutral v
+  | _, .isSegmentTree h => h
+  | _, .mkSegmentTree => isSegmentTree_mkSegmentTree
+  | _, .mkEmpty => isSegmentTree_mkEmpty
+  | _, .modify h => h.out.modify ..
+
+end Impl
+
+public theorem isSegmentTree_tree {op : α → α → α} {neutral : α} [Std.LawfulRightIdentity op neutral]
+    (t : SegmentTree op neutral n) : Impl.IsSegmentTree op neutral t.tree :=
+  t.wf.out
+
+end TCR.SegmentTree
